coq/ZF/Meta/Decl/Axiom/Power.v
@@ -1,0 +1,30 @@
+Require Import Coq.Lists.List.
+Require Import Coq.Strings.String.
+
+Require Import ZF.Meta.Env.
+Require Import ZF.Meta.Syntax.
+Require Import ZF.Meta.Term.Decl.
+Require Import ZF.Meta.Ty.
+
+Import ListNotations.
+
+(* forall a, exists b, forall x, x :< b <-> x <= a                              *)
+Definition Power : DeclT :=
+  {| paraT := []
+  ;  resT  := TyProp
+  ;  bodyT :=
+      All VarTySet
+        (Ex VarTySet
+          (All VarTySet
+            (Iff
+              (Elem (Var 0) (Var 1))
+              (Leq (Var 0) (Var 2)))))
+  |}.
+
+Definition imports : Env := Env.empty.
+
+Definition exports : Env := Env.fromListT
+  [ ("Power"%string, Power)
+  ].
+
+Definition env : Env := Env.union imports exports.
